theory/x64Semantics.thy
@@ -3,7 +3,7 @@ section \<open> x64 Semantics \<close>
 theory x64Semantics
 imports
   Main
-  rBPFCommType Val Mem x64Syntax x64Disassembler x64Assembler
+  rBPFCommType Val Mem x64Syntax x64Disassembler x64Assembler vm rBPFSem
 begin
 
 (*axiomatization x64_decode :: "nat \<Rightarrow> u8 list \<Rightarrow> (nat * instruction) option"*)
@@ -23,38 +23,26 @@ fun undef_regs :: "preg list \<Rightarrow> regset \<Rightarrow> regset" where
 "undef_regs [] rs = rs" |
 "undef_regs (r#l') rs = undef_regs l' (rs#r <- 0)"
 
-datatype outcome = Next u64 regset mem | Stuck
+datatype outcome = Next u64 regset mem stack_state | Stuck
 
-definition exec_ret :: "memory_chunk \<Rightarrow> mem \<Rightarrow> regset \<Rightarrow> outcome" where
-"exec_ret chunk m rs = (
-  let nsp =  (rs (IR SP)) + (u64_of_memory_chunk chunk) in
-    case Mem.loadv M64 m (Vlong nsp) of
-    None \<Rightarrow> Stuck |
-    Some ra \<Rightarrow> (
-      case ra of
-      Vlong v \<Rightarrow> let rs1 = rs#(IR SP) <- nsp in
-                  Next v rs1 m |
-      _ \<Rightarrow> Stuck)
-)"
-
-definition exec_pop :: "usize \<Rightarrow> u64 \<Rightarrow> memory_chunk \<Rightarrow> mem \<Rightarrow> regset \<Rightarrow> ireg \<Rightarrow> outcome" where
-"exec_pop pc sz chunk m rs rd = (
+definition exec_pop :: "usize \<Rightarrow> u64 \<Rightarrow> memory_chunk \<Rightarrow> mem \<Rightarrow> stack_state \<Rightarrow> regset \<Rightarrow> ireg \<Rightarrow> outcome" where
+"exec_pop pc sz chunk m ss rs rd = (
   let nsp = (rs (IR SP)) + (u64_of_memory_chunk chunk) in
     let addr = (rs (IR SP)) in
       case Mem.loadv chunk m (Vptr sp_block addr) of
         None \<Rightarrow> Stuck |
         Some x => 
           (case x of Vlong v \<Rightarrow> let rs1 =rs # (IR SP) <- nsp  in
-          Next (pc + sz) (rs1#(IR rd) <- v ) m |
+          Next (pc + sz) (rs1#(IR rd) <- v ) m ss |
                      _ \<Rightarrow> Stuck)
 )"
 
-definition exec_push :: "usize \<Rightarrow> u64 \<Rightarrow> memory_chunk \<Rightarrow> mem \<Rightarrow> regset \<Rightarrow> usize \<Rightarrow> outcome" where
-"exec_push pc sz chunk m rs v = ( 
+definition exec_push :: "usize \<Rightarrow> u64 \<Rightarrow> memory_chunk \<Rightarrow> mem \<Rightarrow> stack_state \<Rightarrow> regset \<Rightarrow> usize \<Rightarrow> outcome" where
+"exec_push pc sz chunk m ss rs v = ( 
   let nsp = (rs (IR SP)) - (u64_of_memory_chunk chunk) in
       case Mem.storev chunk m (Vptr sp_block nsp) (Vlong v) of
         None \<Rightarrow> Stuck |
-        Some m' => Next (pc + sz) (rs#(IR SP) <- nsp) m'
+        Some m' => Next (pc + sz) (rs#(IR SP) <- nsp) m' ss
 )"
 
 definition of_optbool :: " bool \<Rightarrow> u64" where
@@ -97,24 +85,55 @@ definition eval_addrmode64 :: "addrmode \<Rightarrow> regset \<Rightarrow> u64" 
     + (scast const)) 
 )"
 
-definition exec_load :: "usize \<Rightarrow> u64 \<Rightarrow> memory_chunk \<Rightarrow> mem \<Rightarrow> addrmode \<Rightarrow> regset \<Rightarrow> preg \<Rightarrow> outcome" where
-"exec_load pc sz chunk m a rs rd = (
+definition exec_load :: "usize \<Rightarrow> u64 \<Rightarrow> memory_chunk \<Rightarrow> mem \<Rightarrow> stack_state \<Rightarrow> addrmode \<Rightarrow> regset \<Rightarrow> preg \<Rightarrow> outcome" where
+"exec_load pc sz chunk m ss a rs rd = (
   let addr =  eval_addrmode64 a rs in
     case Mem.loadv chunk m (Vlong addr) of
       None \<Rightarrow> Stuck | 
       Some ra \<Rightarrow> 
-        (case ra of Vlong v \<Rightarrow> Next (pc+sz) (rs#rd <- v) m | 
+        (case ra of Vlong v \<Rightarrow> Next (pc+sz) (rs#rd <- v) m ss | 
                           _ \<Rightarrow> Stuck)
 )"
 
 (*preg list?*)
-definition exec_store :: "usize \<Rightarrow> u64 \<Rightarrow> memory_chunk \<Rightarrow> mem \<Rightarrow> addrmode \<Rightarrow> regset \<Rightarrow> preg \<Rightarrow> outcome" where
-"exec_store pc sz chunk m a rs r1 = (
+definition exec_store :: "usize \<Rightarrow> u64 \<Rightarrow> memory_chunk \<Rightarrow> mem \<Rightarrow> stack_state \<Rightarrow> addrmode \<Rightarrow> regset \<Rightarrow> preg \<Rightarrow> outcome" where
+"exec_store pc sz chunk m ss a rs r1 = (
   let addr =  eval_addrmode64 a rs in (
     case Mem.storev chunk m (Vlong addr) (Vlong (rs r1)) of
       None \<Rightarrow> Stuck |
-      Some m' \<Rightarrow> Next (pc+ sz) rs m'
+      Some m' \<Rightarrow> Next (pc+ sz) rs m' ss
   )
+)"
+(*
+definition exec_call :: "usize \<Rightarrow> u64 \<Rightarrow> memory_chunk \<Rightarrow> mem \<Rightarrow> stack_state \<Rightarrow> regset \<Rightarrow> preg \<Rightarrow> outcome" where
+"exec_call pc sz chunk m ss rs r1 = (
+  let nsp = (rs (IR SP))-(u64_of_memory_chunk chunk) in (
+      case Mem.storev M64 m (Vptr sp_block nsp) (Vlong (rs r1)) of
+        None \<Rightarrow> Stuck |
+        Some m' \<Rightarrow> let rs1 = rs#(IR SP) <- nsp in
+                    Next (rs r1) rs1 m' ss
+))"*)
+
+
+definition exec_call :: "usize \<Rightarrow> u64 \<Rightarrow> memory_chunk \<Rightarrow> mem \<Rightarrow> stack_state \<Rightarrow> regset \<Rightarrow> u32 \<Rightarrow> outcome" where
+"exec_call pc sz chunk m ss rs n = (
+  let nsp = (rs (IR SP))-(u64_of_memory_chunk chunk) in (
+      case Mem.storev M64 m (Vptr sp_block nsp) (Vlong (ucast n)) of
+        None \<Rightarrow> Stuck |
+        Some m' \<Rightarrow> let rs1 = rs#(IR SP) <- nsp in
+                    Next (ucast n) rs1 m' ss
+))"
+
+definition exec_ret :: "memory_chunk \<Rightarrow> mem \<Rightarrow> stack_state \<Rightarrow> regset \<Rightarrow> outcome" where
+"exec_ret chunk m ss rs = (
+  let nsp =  (rs (IR SP)) + (u64_of_memory_chunk chunk) in
+    case Mem.loadv M64 m (Vptr sp_block nsp) of
+    None \<Rightarrow> Stuck |
+    Some ra \<Rightarrow> (
+      case ra of
+      Vlong v \<Rightarrow> let rs1 = rs#(IR SP) <- nsp in
+                  Next v rs1 m ss |
+      _ \<Rightarrow> Stuck)
 )"
 
 
@@ -158,41 +177,42 @@ definition eval_testcond :: "testcond \<Rightarrow> regset \<Rightarrow> bool op
 )"*)
 
 (*Pjmp       d    \<Rightarrow> Next (scast d) rs m*)
-definition exec_instr :: "instruction \<Rightarrow> u64 \<Rightarrow> u64 \<Rightarrow> regset \<Rightarrow> mem \<Rightarrow> outcome" where
-"exec_instr i sz pc rs m = (\<comment> \<open> sz is the binary size (n-byte) of current instruction  \<close>
+definition exec_instr :: "instruction \<Rightarrow> u64 \<Rightarrow> u64 \<Rightarrow> regset \<Rightarrow> mem \<Rightarrow> stack_state \<Rightarrow> outcome" where
+"exec_instr i sz pc rs m ss = (\<comment> \<open> sz is the binary size (n-byte) of current instruction  \<close>
   case i of
-  Paddq_rr  rd r1 \<Rightarrow> Next (pc + sz) ((rs#(IR rd) <- (rs (IR rd) + rs (IR r1)))) m |
-  Pret            \<Rightarrow> exec_ret M64 m rs |
-  Ppopl     rd    \<Rightarrow> exec_pop pc sz M64 m rs rd |
-  Ppushl_r  r1    \<Rightarrow> exec_push pc sz M64 m rs (rs (IR r1)) |
-  Pmovq_rr rd r1  \<Rightarrow> Next (pc + sz) (rs#(IR rd) <- (rs (IR r1))) m |
+  Paddq_rr  rd r1 \<Rightarrow> Next (pc + sz) ((rs#(IR rd) <- (rs (IR rd) + rs (IR r1)))) m ss |
+  Pret            \<Rightarrow> exec_ret M64 m ss rs |
+  Ppopl     rd    \<Rightarrow> exec_pop pc sz M64 m ss rs rd |
+  Ppushl_r  r1    \<Rightarrow> exec_push pc sz M64 m ss rs (rs (IR r1)) |
+  Pmovq_rr rd r1  \<Rightarrow> Next (pc + sz) (rs#(IR rd) <- (rs (IR r1))) m ss|
   Pmulq_r   r1    \<Rightarrow> let rs1 = rs#(IR RAX) <- ((rs (IR RAX))*(rs (IR r1))) in
-                     Next (pc + sz) (rs1#(IR RDX) <-( (rs (IR RAX))*(rs (IR r1)) div (2 ^ 32))) m |
+                     Next (pc + sz) (rs1#(IR RDX) <-( (rs (IR RAX))*(rs (IR r1)) div (2 ^ 32))) m ss|
   Pjcc      t d    \<Rightarrow> (case eval_testcond t rs of Some b \<Rightarrow> 
-                          if b then Next (scast d) rs m 
-                          else Next (pc+sz) rs m | 
+                          if b then Next (scast d) rs m ss
+                          else Next (pc+sz) rs m ss | 
                         None \<Rightarrow> Stuck) |
-  Pcmpq_rr rd r1 \<Rightarrow> Next (pc+sz)(compare_longs (rs (IR r1)) (rs (IR rd)) rs) m |
-  Pmovq_ri rd n  \<Rightarrow> Next (pc + sz) (rs#(IR rd) <- n) m |
-  Pmov_mr  a r1 c \<Rightarrow> exec_load  pc sz c m a rs (IR r1) |                    \<comment> \<open> store reg to mem \<close>
+  Pcmpq_rr rd r1 \<Rightarrow> Next (pc+sz)(compare_longs (rs (IR r1)) (rs (IR rd)) rs) m ss |
+  Pmovq_ri rd n  \<Rightarrow> Next (pc + sz) (rs#(IR rd) <- n) m ss |
+  Pmov_mr  a r1 c \<Rightarrow> exec_load pc sz c m ss a rs (IR r1) |                    \<comment> \<open> store reg to mem \<close>
   Pxchgq_rr rd r1 \<Rightarrow> let tmp = rs (IR rd) in
                      let rs1 = (rs#(IR rd)<- (rs (IR r1))) in
-                       Next (pc + sz) (rs1#(IR r1)<- tmp) m |
-  Pshlq_r   rd    \<Rightarrow> Next (pc + sz) (rs#(IR rd) <- ((rs (IR rd))<< (unat (and ( (ucast (rs(IR RCX)))::u32) (63::u32))))) m |
-  Pshrq_r   rd    \<Rightarrow> Next (pc + sz) (rs#(IR rd) <- ((rs (IR rd))>> (unat (and ( (ucast (rs(IR RCX)))::u32) (63::u32))))) m |
-  Psarq_r   rd    \<Rightarrow> Next (pc + sz) (rs#(IR rd) <- (ucast (((scast (rs (IR rd)))::i64) >> (unat (and ( (ucast (rs(IR RCX)))::u32) (63::u32)))))) m |
-  Pmov_rm  rd a c \<Rightarrow> exec_store pc sz c m a rs (IR rd) 
+                       Next (pc + sz) (rs1#(IR r1)<- tmp) m ss |
+  Pshlq_r   rd    \<Rightarrow> Next (pc + sz) (rs#(IR rd) <- ((rs (IR rd))<< (unat (and ( (ucast (rs(IR RCX)))::u32) (63::u32))))) m ss |
+  Pshrq_r   rd    \<Rightarrow> Next (pc + sz) (rs#(IR rd) <- ((rs (IR rd))>> (unat (and ( (ucast (rs(IR RCX)))::u32) (63::u32))))) m ss |
+  Psarq_r   rd    \<Rightarrow> Next (pc + sz) (rs#(IR rd) <- (ucast (((scast (rs (IR rd)))::i64) >> (unat (and ( (ucast (rs(IR RCX)))::u32) (63::u32)))))) m ss |
+  Pmov_rm  rd a c \<Rightarrow> exec_store pc sz c m ss a rs (IR rd) |
+  Pcall_i   n   \<Rightarrow> exec_call pc sz M64 m ss rs n
 )"
-
+(*Pcall_r   r1    \<Rightarrow> exec_call pc sz M64 m ss rs (IR r1)*)
 
 fun x64_sem :: "nat \<Rightarrow> x64_bin \<Rightarrow> outcome \<Rightarrow> outcome" where
 "x64_sem 0 _ st = st" |
 "x64_sem (Suc n) l Stuck = Stuck"|
-"x64_sem (Suc n) l (Next pc rs m) = (
+"x64_sem (Suc n) l (Next pc rs m ss) = (
   case x64_decode (unat pc) l of
   None \<Rightarrow> Stuck |
   Some (sz, ins) \<Rightarrow>
-    x64_sem n l (exec_instr ins (of_nat sz) pc rs m)
+    x64_sem n l (exec_instr ins (of_nat sz) pc rs m ss)
 )"
 
 lemma x64_sem_add_stuck : 
@@ -206,20 +226,20 @@ lemma x64_sem_add_stuck :
 
 lemma x64_sem_add: 
   "x64_sem (m+n) x64_prog xst = xst' \<Longrightarrow>
-    xst = (Next pc rs ms) \<Longrightarrow>
+    xst = (Next pc rs ms ss) \<Longrightarrow>
     \<exists> xst1.
     x64_sem m x64_prog xst = xst1 \<and> 
     x64_sem n x64_prog xst1 = xst'"
-  apply (induction m arbitrary: n x64_prog xst xst' pc rs ms)
+  apply (induction m arbitrary: n x64_prog xst xst' pc rs ms ss)
   subgoal by simp
-  subgoal for m n x64_prog xst xst' pc rs ms
+  subgoal for m n x64_prog xst xst' pc rs ms ss
     apply simp
     apply (cases "x64_decode (unat pc) x64_prog"; simp)
     subgoal by (cases n; simp)
     subgoal for ins1
       apply (cases ins1; simp)
       subgoal for sz ins
-        apply (cases "(exec_instr ins (word_of_nat sz) pc rs ms)"; simp)
+        apply (cases "(exec_instr ins (word_of_nat sz) pc rs ms ss)"; simp)
         apply (erule x64_sem_add_stuck)
         done
       done
@@ -228,21 +248,51 @@ lemma x64_sem_add:
 
 type_synonym hybrid_state = "u64 \<times> outcome"
 
+
+definition save_x64_caller::"regset \<Rightarrow> u64 list" where
+"save_x64_caller xrs = [xrs (IR R12), xrs (IR R13), xrs (IR R14), xrs (IR R15)]"
+
+definition save_x64_frame_pointer::"regset \<Rightarrow> u64" where
+"save_x64_frame_pointer xrs = xrs (IR RBP)"
+
+definition upate_x64_stack_pointer::"regset \<Rightarrow> u64 \<Rightarrow> regset" where
+"upate_x64_stack_pointer rs v = (rs#(IR RBP) <-- v)"
+
+definition restore_x64_caller::"regset \<Rightarrow> u64 list \<Rightarrow> u64 \<Rightarrow> regset" where
+"restore_x64_caller rs caller fp = (let rs'= (((((
+            rs#(IR RBP) <-- fp)
+              #(IR R15)  <-- (caller!(3)))
+              #(IR R14)  <-- (caller!(2)))
+              #(IR R13)  <-- (caller!(1)))
+              #(IR R12)  <-- (caller!(0))) in rs')"
+(*
+definition get_target_addr::"regset \<Rightarrow> u8 \<Rightarrow> u64" where
+"get_target_addr xrs xrid = xrs (IR (the (ireg_of_u8 xrid)))"*)
+
 definition one_step:: " (nat \<times> u64 \<times> x64_bin) list \<Rightarrow> hybrid_state\<Rightarrow> hybrid_state" where
 "one_step lt st  \<equiv>
   let pc = fst st; xst = snd st in 
   let (num,off,l) = lt!(unat pc) in
     case xst of
-    Next xpc rs m \<Rightarrow> (
-      if l!1 = (0x39::u8) then 
-        let xst_temp = Next 0 rs m; xst' = x64_sem num l xst_temp in
+    Next xpc rs m ss \<Rightarrow> (   
+       if l!0 = 0xc3 then
+          let (pc', ss', caller,fp) = update_stack2 ss in 
+          let rs' = restore_x64_caller rs caller fp in (pc', Next xpc rs' m ss')
+      else if (l!0 = 0xe8) then 
+        let caller = save_x64_caller rs; fp = save_x64_frame_pointer rs; 
+            rs' = upate_x64_stack_pointer rs (stack_pointer ss) in
+        let ss' = update_stack caller fp (pc+1) ss in
+          (case ss' of None \<Rightarrow> (pc, Stuck) | 
+          Some ra \<Rightarrow> (ucast(the (u32_of_u8_list (tl l))), Next xpc rs' m ra))
+      else if l!1 = (0x39::u8)  then
+        let xst_temp = Next 0 rs m ss; xst' = x64_sem num l xst_temp in
           case xst' of
-          Next xpc' rs' m' \<Rightarrow>
+          Next xpc' rs' m' ss'\<Rightarrow>
             if rs' (CR ZF) = 1 then (off+pc, xst')
             else (pc+1, xst') |
-          Stuck \<Rightarrow> (pc, Stuck)
+          Stuck \<Rightarrow> (pc, Stuck)      
       else
-        let xst_temp = Next 0 rs m; xst' = x64_sem num l xst_temp in
+        let xst_temp = Next 0 rs m ss; xst' = x64_sem num l xst_temp in
           (pc+1, xst'))
     | Stuck \<Rightarrow> (pc,Stuck)"
 
