theory/JITPer_jump.thy
@@ -9,7 +9,7 @@ begin
 
 
 lemma jccq_subgoal_rr_aux3:"bins = BPF_JUMP cond dst (SOReg src) d \<Longrightarrow> 
-  sbpf_step prog (SBPF_OK pc rs m) = (SBPF_OK pc' rs' m') \<Longrightarrow> 
+  sbpf_step prog (SBPF_OK pc rs m s) = (SBPF_OK pc' rs' m' s') \<Longrightarrow> 
   prog!(unat pc) = bins \<Longrightarrow>
   \<forall> r. rs' r = rs r"
   apply(cases bins,simp_all)
@@ -19,8 +19,8 @@ lemma jccq_subgoal_rr_aux3:"bins = BPF_JUMP cond dst (SOReg src) d \<Longrightar
 
 lemma mem_is_not_changed_by_jump:
   "prog!(unat pc1) = BPF_JUMP cond dst (SOReg src) d \<Longrightarrow> 
-  s2 = sbpf_step prog s1 \<Longrightarrow> s1 = (SBPF_OK pc1 rs1 m1) \<Longrightarrow> 
-  s2 = (SBPF_OK pc2 rs2 m2) \<Longrightarrow> m1 = m2"
+  s2 = sbpf_step prog s1 \<Longrightarrow> s1 = (SBPF_OK pc1 rs1 m1 ss1) \<Longrightarrow> 
+  s2 = (SBPF_OK pc2 rs2 m2 ss2) \<Longrightarrow> m1 = m2"
   apply(cases "prog!(unat pc1)", simp_all)
   apply(split if_splits,simp_all)
   apply(split if_splits,simp_all)
@@ -33,12 +33,12 @@ lemma jcc_subgoal_rr_generic:
   assumes a0:"bins = BPF_JUMP cond dst (SOReg src) d" and
        a1:"per_jit_jcc cond dst src (scast d) = Some (num, off, l_bin)" and
        a3:"x64_decode 0 l_bin = Some (n, xins)" and
-       a4:"sbpf_step prog (SBPF_OK pc rs m) = (SBPF_OK pc' rs' m')" and
-       a5:"Next spc' reg' xm' = exec_instr xins sz spc reg xm" and
-       a6:"match_state (SBPF_OK pc rs m) (pc, Next spc reg xm) " and
+       a4:"sbpf_step prog (SBPF_OK pc rs m ss) = (SBPF_OK pc' rs' m' ss')" and
+       a5:"Next spc' reg' xm' xss' = exec_instr xins sz spc reg xm xss" and
+       a6:"match_state (SBPF_OK pc rs m ss) (pc, Next spc reg xm xss) " and
        a7:"prog!(unat pc) = bins" and
        a8:"cond = Eq"
-  shows "match_state (SBPF_OK pc' rs' m') (pc', Next spc' reg' xm') "
+  shows "match_state (SBPF_OK pc' rs' m' ss') (pc', Next spc' reg' xm' xss') "
 proof -
   let "?tcond" = "Cond_e"
   have b0_1:"l_bin = (let ins1 = Pcmpq_rr (bpf_to_x64_reg dst) (bpf_to_x64_reg src) in
@@ -60,14 +60,20 @@ proof -
   have b9:"match_mem m' xm'" using match_state_def a6 a5 b0 apply (simp add: exec_instr_def) 
     using a4 mem_is_not_changed_by_jump
     by (metis a0 a7 bpf_instruction.distinct(63))
+  have "ss=xss" using match_state_def a6 by simp 
+  moreover have "ss' = ss" using a0 a4 a7 apply(cases "prog!(unat pc)",simp_all) subgoal for x161
+      by (smt (z3) bpf_instruction.simps(376) sbpf_state.inject(1) sbpf_state.simps(6) snd_op.simps(6)) 
+    done
+  moreover have "xss' = xss" using b0 a5 by(unfold exec_instr_def,simp_all)
+    ultimately have "ss' = xss'" by meson 
   thus ?thesis using b4  match_state_def b8 b9 match_reg_def by fastforce
 qed
 
 lemma jump_one_step:
   assumes a0:"s' = sbpf_step prog s" and
-  a1:"s = (SBPF_OK pc rs m)" and
-  a2:"s' = (SBPF_OK pc' rs' m')" and
-  a3:"xst = (Next xpc xrs xm)" and
+  a1:"s = (SBPF_OK pc rs m ss)" and
+  a2:"s' = (SBPF_OK pc' rs' m' ss')" and
+  a3:"xst = (Next xpc xrs xm xss)" and
   a4:"match_state s (pc,xst)" and
   a5:"jitper prog = Some x64_prog" and                      
   a6:"prog \<noteq> [] \<and> unat pc < length prog \<and> unat pc \<ge> 0" and
@@ -104,12 +110,25 @@ proof-
       apply(cases cond,simp_all)
       apply(unfold x64_encode_def,simp_all) by auto
 
-    have "?st = snd (let xst_temp = Next 0 xrs xm; xst' = x64_sem num l xst_temp in
-        case xst' of Next xpc' rs' m' \<Rightarrow>
+    have e3_1:"l!0 \<notin> {0xc3,0xe8}" using c_aux c3 c1_1 
+      apply(unfold per_jit_jcc_def Let_def) 
+      apply(cases cond,simp_all)
+      apply(unfold x64_encode_def,simp_all)
+      apply(unfold construct_rex_to_u8_def bitfield_insert_u8_def Let_def u8_of_bool_def,simp_all)
+      apply(cases "and (u8_of_ireg (bpf_to_x64_reg dst)) (8::8 word) \<noteq> (0::8 word)",simp_all)
+       apply(cases "and (u8_of_ireg (bpf_to_x64_reg src)) (8::8 word) \<noteq> (0::8 word)",simp_all)
+        apply auto[1]
+       apply auto[1]
+      apply(cases " and (u8_of_ireg (bpf_to_x64_reg src)) (8::8 word) \<noteq> (0::8 word)",simp_all)
+       apply auto[1]
+      by auto
+    have e3_2:"l!0 \<noteq> 0xc3 \<and> l!0 \<noteq> 0xe8 \<and> l!1 = 0x39" using e3_0 e3_1 by simp
+    have "?st = snd (let xst_temp = Next 0 xrs xm xss; xst' = x64_sem num l xst_temp in
+        case xst' of Next xpc' rs' m' xss' \<Rightarrow>
           if rs' (CR ZF) = 1 then (off+pc, xst')
           else (pc+1, xst') |
-         Stuck \<Rightarrow> (pc, Stuck))" using c2_1 a3 one_step_def c_aux e3_0 by simp
-    hence e3_1:"?st = x64_sem num ?l_bin (Next 0 xrs xm)" using c2_1 c_aux one_step_def a3
+         Stuck \<Rightarrow> (pc, Stuck))" using c2_1 a3 one_step_def c_aux e3_0 e3_1 by simp
+    hence e3_1:"?st = x64_sem num ?l_bin (Next 0 xrs xm xss)" using c2_1 c_aux one_step_def a3
       by (smt (verit, ccfv_threshold) c2 outcome.exhaust outcome.simps(4) outcome.simps(5) snd_conv) 
 
     let "?l_bin1" = "x64_encode (Pcmpq_rr (bpf_to_x64_reg dst) (bpf_to_x64_reg src))"
@@ -123,11 +142,11 @@ proof-
       by (metis c1 d0 list_in_list_concat x64_encode_decode_consistency)
     then obtain xins1 sz1 where d1:"x64_decode 0 ?l_bin = Some (sz1, xins1)" by auto
     have d2:"(sz1,xins1) = (3, Pcmpq_rr (bpf_to_x64_reg dst) (bpf_to_x64_reg src))"  using d0_1 x64_encode_decode_consistency d1 x64_encode_def by fastforce
-    have c4:"?st = exec_instr xins1 (of_nat sz1) 0 xrs xm" using c3_1 d2 c1 c2 a3 d1 e3_1 by auto 
-    have c6:"\<exists> xrs' xpc' xm'. ?st = Next xpc' xrs' xm'" using exec_instr_def spec c4 d2 by simp
-    obtain xrs' xpc' xm' where c7:"?st = Next xpc' xrs' xm'" using c6 by auto
+    have c4:"?st = exec_instr xins1 (of_nat sz1) 0 xrs xm xss" using c3_1 d2 c1 c2 a3 d1 e3_1 by auto 
+    have c6:"\<exists> xrs' xpc' xm' xss'. ?st = Next xpc' xrs' xm' xss'" using exec_instr_def spec c4 d2 by simp
+    obtain xrs' xpc' xm' xss' where c7:"?st = Next xpc' xrs' xm' xss'" using c6 by auto
   
-    have e0_1:"exec_instr xins1 (of_nat sz1) 0 xrs xm = Next (0+(of_nat sz1))(compare_longs (xrs (IR (bpf_to_x64_reg src))) (xrs (IR (bpf_to_x64_reg dst))) xrs) xm"
+    have e0_1:"exec_instr xins1 (of_nat sz1) 0 xrs xm xss = Next (0+(of_nat sz1))(compare_longs (xrs (IR (bpf_to_x64_reg src))) (xrs (IR (bpf_to_x64_reg dst))) xrs) xm xss"
       using  exec_instr_def d2 a3 by simp
      
     hence e0:"let x = xrs (IR (bpf_to_x64_reg src)); y = xrs (IR (bpf_to_x64_reg dst)) in
@@ -142,12 +161,12 @@ proof-
     have e2:"xrs (IR (bpf_to_x64_reg dst)) \<noteq> xrs (IR (bpf_to_x64_reg src)) \<longrightarrow>xrs' (CR ZF) = 0" 
       by (smt (verit, del_insts) crbit.distinct(1) crbit.distinct(5) crbit.distinct(7) e0 fun_upd_apply preg.inject(2) x64Semantics.of_optbool_def)
 
-    have cn_1:"match_state s (pc,(Next 0 xrs xm))" using a4 match_state_eqiv a3 by blast  
-    have cn:"x64_sem num l (Next 0 xrs xm) = ?st \<and> match_state s' (pc',?st)"
+    have cn_1:"match_state s (pc,(Next 0 xrs xm xss))" using a4 match_state_eqiv a3 by blast  
+    have cn:"x64_sem num l (Next 0 xrs xm xss) = ?st \<and> match_state s' (pc',?st)"
       using jcc_subgoal_rr_generic a0 a1 a2 c7 per_jit_jcc_def a8  c1_1 d1 c2 e3_1 c3_0 c3 c_aux e0_1 c4 cn_1 by metis
       
-    have "x64_sem1 1 x64_prog (pc,xst) = (pc', Next xpc' xrs' xm')"
-      using a8 e1 e2 cn a0 a1 a2 a3 a4 a5 a6 x64_sem1_pc_aux1 c_aux match_state_eqiv e3_0 c7 x64_sem1_pc_aux2 by auto
+    have "x64_sem1 1 x64_prog (pc,xst) = (pc', Next xpc' xrs' xm' xss')"
+      using a8 e1 e2 cn a0 a1 a2 a3 a4 a5 a6 c_aux match_state_eqiv c7 x64_sem1_pc_aux2 e3_2 by simp
     then show ?thesis using a8 c2 match_state_eqiv c7 cn by fastforce
     qed
 
