theory/JITPer_mul_rax.thy
@@ -8,9 +8,9 @@ imports
 begin
 
 lemma mulq_one_step_match_reg:
-  " (SBPF_OK pc' rs' m') = sbpf_step prog (SBPF_OK pc rs m) \<Longrightarrow>
-    xst = (Next xpc xrs xm) \<Longrightarrow>
-    match_state (SBPF_OK pc rs m) (pc,xst) \<Longrightarrow>
+  " (SBPF_OK pc' rs' m' ss') = sbpf_step prog (SBPF_OK pc rs m ss) \<Longrightarrow>
+    xst = (Next xpc xrs xm xss) \<Longrightarrow>
+    match_state (SBPF_OK pc rs m ss) (pc,xst) \<Longrightarrow>
     prog \<noteq> [] \<and> unat pc < length prog \<and> unat pc \<ge> 0 \<Longrightarrow>
     prog!(unat pc) = BPF_ALU64 BPF_MUL dst (SOReg src) \<Longrightarrow>
     (bpf_to_x64_reg dst) = RAX \<Longrightarrow>
@@ -24,9 +24,9 @@ lemma mulq_one_step_match_reg:
   by (metis bpf_to_x64_reg_corr reg_r11_consist)
 
 lemma mulq_one_step_match_mem:
-  " (SBPF_OK pc' rs' m') = sbpf_step prog (SBPF_OK pc rs m) \<Longrightarrow>
-    xst = (Next xpc xrs xm) \<Longrightarrow>
-    match_state (SBPF_OK pc rs m) (pc,xst) \<Longrightarrow>
+  " (SBPF_OK pc' rs' m' ss') = sbpf_step prog (SBPF_OK pc rs m ss) \<Longrightarrow>
+    xst = (Next xpc xrs xm xss) \<Longrightarrow>
+    match_state (SBPF_OK pc rs m ss) (pc,xst) \<Longrightarrow>
     prog \<noteq> [] \<and> unat pc < length prog \<and> unat pc \<ge> 0 \<Longrightarrow>
     prog!(unat pc) = BPF_ALU64 BPF_MUL dst (SOReg src) \<Longrightarrow>
     (bpf_to_x64_reg dst) = RAX \<Longrightarrow>
@@ -42,9 +42,9 @@ lemma mulq_one_step_match_mem:
   
   
 lemma mulq_one_step_match_stack:
-  " (SBPF_OK pc' rs' m') = sbpf_step prog (SBPF_OK pc rs m) \<Longrightarrow>
-    xst = (Next xpc xrs xm) \<Longrightarrow>
-    match_state (SBPF_OK pc rs m) (pc,xst) \<Longrightarrow>
+  " (SBPF_OK pc' rs' m' ss') = sbpf_step prog (SBPF_OK pc rs m ss) \<Longrightarrow>
+    xst = (Next xpc xrs xm xss) \<Longrightarrow>
+    match_state (SBPF_OK pc rs m ss) (pc,xst) \<Longrightarrow>
     prog \<noteq> [] \<and> unat pc < length prog \<and> unat pc \<ge> 0 \<Longrightarrow>
     prog!(unat pc) = BPF_ALU64 BPF_MUL dst (SOReg src) \<Longrightarrow>
     (bpf_to_x64_reg dst) = RAX \<Longrightarrow>
@@ -59,11 +59,37 @@ lemma mulq_one_step_match_stack:
     "
   by (simp add: match_state_def match_stack_def eval_alu_def eval_reg_def)
 
+
+lemma encode_aux:"(x64_encode (Pmovq_rr R11 (bpf_to_x64_reg src))@(x64_encode (Ppushl_r RDX)) @ (x64_encode (Pmulq_r R11)) @ (x64_encode (Ppopl RDX)))!0 \<notin> {0xc3, 0xe8}"
+ subgoal apply(unfold per_jit_mul_reg64_def x64_encode_def)
+   apply(unfold construct_rex_to_u8_def bitfield_insert_u8_def Let_def u8_of_bool_def,simp_all)
+   apply(cases "and (u8_of_ireg (bpf_to_x64_reg src)) (8::8 word)",simp_all)
+   subgoal for n apply(cases " word_of_nat n \<noteq> (0::8 word)",simp_all)
+     done
+   done
+  done
+
+
+
+lemma mulq_one_step_match_stack2:
+  " (SBPF_OK pc' rs' m' ss') = sbpf_step prog (SBPF_OK pc rs m ss) \<Longrightarrow>
+    xst = (Next xpc xrs xm xss) \<Longrightarrow>
+    match_state (SBPF_OK pc rs m ss) (pc,xst) \<Longrightarrow>
+    prog \<noteq> [] \<and> unat pc < length prog \<and> unat pc \<ge> 0 \<Longrightarrow>
+    prog!(unat pc) = BPF_ALU64 BPF_MUL dst (SOReg src) \<Longrightarrow>
+    xss=ss'"
+  apply(cases"prog!(unat pc)",simp_all)
+  subgoal for x91 
+    apply(cases "eval_alu BPF_MUL dst (SOReg src) rs",simp_all)
+    apply(unfold match_state_def,simp_all)
+    done
+  done
+
 lemma mulq_one_step_rax:
 assumes a0:"s' = sbpf_step prog s" and
-  a1:"s = (SBPF_OK pc rs m)" and
-  a2:"s' = (SBPF_OK pc' rs' m')" and
-  a3:"xst = (Next xpc xrs xm)" and
+  a1:"s = (SBPF_OK pc rs m ss)" and
+  a2:"s' = (SBPF_OK pc' rs' m' ss')" and
+  a3:"xst = (Next xpc xrs xm xss)" and
   a4:"match_state s (pc,xst)" and
   a5:"jitper prog = Some x64_prog" and                      
   a6:"prog \<noteq> [] \<and> unat pc < length prog \<and> unat pc \<ge> 0" and
@@ -89,7 +115,9 @@ shows "\<exists> xst'. x64_sem1 1 x64_prog (pc,xst) = (pc',xst') \<and>
        prefer 2
       subgoal using per_jit_mul_reg64_def a9 by simp
       apply(subgoal_tac "(x64_encode (Pmovq_rr R11 (bpf_to_x64_reg src))@(x64_encode (Ppushl_r RDX)) @ (x64_encode (Pmulq_r R11)) @ (x64_encode (Ppopl RDX)))!1 \<noteq> 0x39")
-        prefer 2 subgoal using per_jit_mul_reg64_def x64_encode_def by auto
+       prefer 2 subgoal using per_jit_mul_reg64_def x64_encode_def by auto
+      apply(subgoal_tac "(x64_encode (Pmovq_rr R11 (bpf_to_x64_reg src))@(x64_encode (Ppushl_r RDX)) @ (x64_encode (Pmulq_r R11)) @ (x64_encode (Ppopl RDX)))!0 \<notin> {0xc3, 0xe8}")
+      prefer 2 using encode_aux apply simp
       subgoal
         unfolding a3
         apply simp
@@ -207,10 +235,6 @@ shows "\<exists> xst'. x64_sem1 1 x64_prog (pc,xst) = (pc',xst') \<and>
         unfolding a1 a2
         apply (simp add: match_state_def)
         apply (rule conjI)
-
-
-
-
 (* 4.1  match_reg *)
         subgoal using mulq_one_step_match_reg a0 a1 a2 a3 a4 a6 a8 a9
           by simp
@@ -219,7 +243,8 @@ shows "\<exists> xst'. x64_sem1 1 x64_prog (pc,xst) = (pc',xst') \<and>
 (* 4.2  match_mem *)
         subgoal using mulq_one_step_match_mem a0 a1 a2 a3 a4 a6 a8 a9 by simp
 (* 4.2  match_stack *)
-        subgoal using mulq_one_step_match_stack a0 a1 a2 a3 a4 a6 a8 a9 by simp
+        subgoal using mulq_one_step_match_stack a0 a1 a2 a3 a4 a6 a8 a9 apply simp
+          using mulq_one_step_match_stack2 a0 a1 a2 a3 a4 a6 a8 a9 by (metis (no_types, lifting)) 
         done
       done
     done
