theory/JIT_def.thy
@@ -7,7 +7,7 @@ imports
 
 
 begin
-
+(*
 record CallFrame = (*  /// The caller saved registers
     pub caller_saved_registers: [u64; ebpf::SCRATCH_REGS],
 *)
@@ -25,7 +25,7 @@ type_synonym func_key = u32
 type_synonym func_val = u64
 type_synonym func_map = "(func_key, func_val) map"
 
-
+*)
 
 
 
